ProofLibrary/ChaseSequence/Termination/MfaLike.lean
@@ -1,0 +1,30 @@
+import ProofLibrary.ChaseSequence.Termination.Basic
+
+variable {sig : Signature} [DecidableEq sig.P] [DecidableEq sig.C] [DecidableEq sig.V]
+
+def criticalInstance (rs : RuleSet sig) (finite : rs.rules.finite) (special_const : sig.C) : Database sig :=
+  ⟨fun f => f.predicate ∈ rs.predicates ∧ ∀ t, t ∈ f.terms -> t = special_const, by
+    have preds_finite := rs.predicates_finite_of_finite finite
+    rcases preds_finite with ⟨l, nodup, eq⟩
+    exists l.map (fun p => {
+      predicate := p
+      terms := List.repeat special_const (sig.arity p)
+      arity_ok := by rw [List.length_repeat]
+    })
+    constructor
+    . sorry
+    . intro f
+      simp
+      constructor
+      . intro h
+        rcases h with ⟨p, p_mem, f_eq⟩
+        rw [← f_eq]
+        simp [Set.element]
+        rw [eq] at p_mem
+        constructor
+        . exact p_mem
+        . intro t
+          sorry
+      sorry
+  ⟩
+
