ProofLibrary/ChaseSequence/Universality.lean
@@ -6,7 +6,7 @@ variable {obs : ObsoletenessCondition sig} {kb : KnowledgeBase sig}
 abbrev InductiveHomomorphismResult (ct : ChaseTree obs kb) (m : FactSet sig) (depth : Nat) := {pair : (List Nat) × (GroundTermMapping sig) // pair.1.length = depth ∧ (ct.tree.get pair.1).is_none_or (fun fs => pair.2.isHomomorphism fs.fact m) }
 
 -- TODO: split up the following definition (rather the proofs inside) to get rid of heartbeat increase
-set_option maxHeartbeats 300000
+set_option maxHeartbeats 400000
 
 noncomputable def inductive_homomorphism_with_prev_node_and_trg (ct : ChaseTree obs kb) (m : FactSet sig) (m_is_model : m.modelsKb kb) (prev_depth : Nat) (prev_result : InductiveHomomorphismResult ct m prev_depth) (prev_node_unwrapped : ChaseNode obs kb.rules) (prev_node_eq : ct.tree.get prev_result.val.fst = some prev_node_unwrapped) (trg_ex : exists_trigger_list obs kb.rules prev_node_unwrapped (ct.tree.children prev_result.val.fst)) : InductiveHomomorphismResult ct m (prev_depth + 1) :=
   let prev_path := prev_result.val.fst
